copy more files

Capture/Std/Hedge.lean
@@ -1,5 +1,211 @@
+-- A minimum Hedge library that could be added to a standard library,
+-- A hedge looks similar Haskell's rose tree, but has no laziness and is finite in size.
+
+import Lean.Elab.Tactic
+
+import Capture.Std.List
+
 inductive Hedge.Node (α: Type) where
   | mk (label: α) (children: List (Hedge.Node α))
   deriving BEq, Ord, Repr, Hashable
 
 abbrev Hedge α := List (Hedge.Node α)
+
+namespace Hedge
+
+def Node.getLabel (t: Node α): α :=
+  match t with
+  | Node.mk l _ => l
+
+def Node.getChildren (t: Node α): Hedge α :=
+  match t with
+  | Node.mk _ c => c
+
+def node {α: Type} (label: α) (children: Hedge α): Hedge.Node α :=
+  Hedge.Node.mk label children
+
+example: Hedge String := [
+  node "html" [
+    node "head" [
+      node "title" [node "My Title" []]
+    ],
+    node "body" [
+      node "p" [node "First Paragraph" []],
+      node "p" [node "Second Paragraph" []]
+    ]
+  ]
+]
+
+example: Hedge String := [
+  node "html" [
+    node "head" [],
+    node "body" []
+  ]
+]
+
+private def Node.text (s: String) (children: Hedge (Option String)):
+  Hedge.Node (Option String) :=
+  node (Option.some s) children
+
+private def Node.elem (children: Hedge (Option String)):
+  Hedge.Node (Option String) :=
+  node Option.none children
+
+example: Hedge (Option String) := [
+  Node.text "Subject" [Node.text "hello" []],
+  Node.text "From"    [Node.text "me@mail.org" []],
+  Node.text "To"      [Node.elem [Node.text "you@mail.com" []]],
+  Node.text "Attachments" [
+    Node.elem [
+      Node.text "Filename" [Node.text "first.md" []],
+      Node.text "Contents" [Node.text "remember" []],
+    ],
+    Node.elem [
+      Node.text "Filename" [Node.text "next.txt" []],
+      Node.text "Contents" [Node.text "to reply" []],
+    ]
+  ]
+]
+
+mutual
+def Node.hasDecEq [DecidableEq α]: (a b : Node α) → Decidable (Eq a b)
+  | Node.mk la as, Node.mk lb bs =>
+    match decEq la lb with
+    | isFalse nlab => isFalse (by
+        simp only [Node.mk.injEq, not_and]
+        intro h
+        contradiction
+      )
+    | isTrue hlab =>
+      match Node.hasDecEqs as bs with
+      | isFalse nabs => isFalse (by
+          simp only [Node.mk.injEq, not_and]
+          intro _ hab
+          contradiction
+        )
+      | isTrue habs => isTrue (by
+          rw [hlab]
+          rw [habs]
+        )
+def Node.hasDecEqs [DecidableEq α]: (as bs : Hedge α) → Decidable (Eq as bs)
+  | [], [] => isTrue rfl
+  | (a::as), [] => isFalse (by
+      intro h
+      contradiction
+    )
+  | [], (b::bs) => isFalse (by
+      intro h
+      contradiction
+    )
+  | (a::as), (b::bs) =>
+    match Node.hasDecEq a b with
+    | isFalse nab => isFalse (by
+        simp only [List.cons.injEq, not_and]
+        intro _ hab
+        contradiction
+      )
+    | isTrue hab =>
+      match Node.hasDecEqs as bs with
+      | isFalse nabs => isFalse (by
+          intro h
+          cases h
+          contradiction
+        )
+      | isTrue habs => isTrue (hab ▸ habs ▸ rfl)
+end
+
+instance[DecidableEq α] : DecidableEq (Node α) := Node.hasDecEq
+
+local elab "simp_sizeOf" : tactic => do
+  Lean.Elab.Tactic.evalTactic (<- `(tactic|
+    simp only [Node.mk.sizeOf_spec, List.cons.sizeOf_spec, List.nil.sizeOf_spec, Subtype.mk.sizeOf_spec])
+  )
+
+private theorem lt_plus (x y z: Nat):
+  y < z → x + y < x + z := by
+  simp
+
+private theorem take_eq_self_iff (xs : List α) {n : Nat} : xs.take n = xs ↔ xs.length ≤ n :=
+  ⟨fun h ↦ by rw [← h]; simp; omega, List.take_of_length_le⟩
+
+theorem sizeOf_take (n: Nat) (xs: Hedge α):
+  List.take n xs = xs \/ sizeOf (List.take n xs) < sizeOf xs := by
+  rw [take_eq_self_iff]
+  by_cases (List.length xs > n)
+  case pos h =>
+    apply Or.inr
+    induction n generalizing xs with
+    | zero =>
+      simp only [List.take]
+      simp_sizeOf
+      cases xs with
+      | nil =>
+        simp only [List.length_nil, gt_iff_lt, Nat.lt_irrefl] at h
+      | cons x xs =>
+        simp_sizeOf
+        cases x
+        simp_sizeOf
+        omega
+    | succ n' ih =>
+      cases xs with
+      | nil =>
+        simp at h
+      | cons x xs =>
+        simp only [List.take]
+        simp_sizeOf
+        simp only [List.length_cons, gt_iff_lt, Nat.add_lt_add_iff_right] at h
+        apply lt_plus
+        apply ih
+        exact h
+  case neg h =>
+    simp only [gt_iff_lt, Nat.not_lt] at h
+    apply Or.inl
+    assumption
+
+theorem sizeOf_drop (n: Nat) (xs: Hedge α):
+  List.drop n xs = xs \/ sizeOf (List.drop n xs) < sizeOf xs := by
+  have h := List.drop_exists (xs := xs) (n := n)
+  cases h with
+  | intro ys h =>
+  have h' : List.drop n xs = xs <-> List.drop n xs = ys ++ List.drop n xs := by
+    rw [<- h]
+  rw [h']
+  clear h'
+  have h' : sizeOf xs = sizeOf (ys ++ List.drop n xs) := by
+    rw [<- h]
+  rw [h']
+  cases ys with
+  | nil =>
+    simp only [List.nil_append, Nat.lt_irrefl, or_false]
+  | cons y ys =>
+    apply Or.inr
+    apply List.sizeOf_cons
+
+private theorem Node.sizeOf_lt_cons_child {α: Type} (label: α) (x1: Hedge.Node α) (x2: Hedge.Node α) (xs: Hedge α):
+  sizeOf x1 < sizeOf (Hedge.Node.mk label xs)
+  → sizeOf x1 < sizeOf (Hedge.Node.mk label (x2 :: xs)) := by
+  simp
+  intro h
+  omega
+
+theorem Node.sizeOf_children
+  {α : Type}
+  {child : Node α}
+  {label : α}
+  {children : List (Node α)}
+  (h : child ∈ children)
+  : sizeOf child < sizeOf (Hedge.Node.mk label children) := by
+  induction children with
+  | nil =>
+    simp at h
+  | cons x xs ih =>
+    simp at h
+    cases h with
+    | inl h =>
+      rw [h]
+      simp
+      omega
+    | inr h =>
+      apply Hedge.Node.sizeOf_lt_cons_child
+      apply ih
+      assumption
