Capture.lean
@@ -1,2 +1,3 @@
 import Capture.Std
+import Capture.Regex
 import Capture.Grammar
