Capture/Grammar.lean
@@ -1,1 +1,3 @@
+import Capture.Grammar.Lang
 import Capture.Grammar.Start
+import Capture.Grammar.Grammar
