Capture/Grammar/Lang.lean
@@ -1,0 +1,87 @@
+-- We extend the semantics of regular expressions in Capture.Regex.Lang to also include hedge nodes.
+
+import Capture.Std.Hedge
+
+import Capture.Regex.Lang
+
+namespace Lang
+
+-- The denotation of node used in Grammar.Denote
+def node_match {α: Type} (φ: α → Bool) (R: Lang (Hedge.Node α)): Lang (Hedge.Node α) :=
+  fun xs =>
+    match xs with
+    | [Hedge.Node.mk label children] =>
+      φ label /\ R children
+    | _ => False
+
+-- The denotation of node that we would have liked to use, if match was not required for termination proof purposes.
+-- Luckily we still get to use this definition in a lot of proofs.
+def node {α: Type} (φ: α → Bool) (R: Lang (Hedge.Node α)): Lang (Hedge.Node α) :=
+  fun xs => ∃ label children, xs = [Hedge.Node.mk label children] /\ φ label /\ R children
+
+-- We show that the two definitions of denotation of node is equivalent.
+theorem node_is_node_match:
+  node φ R = node_match φ R := by
+  unfold node
+  unfold node_match
+  funext xs
+  cases xs with
+  | nil =>
+    simp only [List.ne_cons_self, false_and, exists_const, exists_false]
+  | cons x xs =>
+    cases xs with
+    | nil =>
+      simp only [List.cons.injEq, and_true, eq_iff_iff]
+      cases x with
+      | mk label children =>
+      simp only [Hedge.Node.mk.injEq]
+      apply Iff.intro
+      case mp =>
+        intro h
+        obtain ⟨label1, children1, ⟨h1, h2⟩, h3⟩ := h
+        subst_vars
+        exact h3
+      case mpr =>
+        intro ⟨h1, h2⟩
+        exists label
+        exists children
+    | cons x' xs =>
+      simp only [List.cons.injEq, reduceCtorEq, and_false, false_and, exists_const, exists_false]
+
+example: Lang (Hedge.Node Nat) := (node (fun x => x = 1) (Lang.or (node (fun x => x = 1) Lang.emptystr) Lang.emptyset))
+
+theorem null_iff_node {α: Type} {p: α → Bool} {children: Lang (Hedge.Node α)}:
+  Lang.null (node p children) <-> False :=
+  Iff.intro nofun nofun
+
+theorem null_node {α: Type} {p: α → Bool} {children: Lang (Hedge.Node α)}:
+  Lang.null (node p children) = False := by
+  rw [null_iff_node]
+
+theorem derive_iff_node {α: Type} {p: α → Bool} {childlang: Lang (Hedge.Node α)} {label: α} {children: Hedge α} {xs: Hedge α}:
+  (Lang.derive (node p childlang) (Hedge.Node.mk label children)) xs <->
+  (Lang.onlyif (p label /\ childlang children) Lang.emptystr) xs := by
+  simp only [Lang.derive]
+  simp only [Lang.onlyif, Lang.emptystr]
+  refine Iff.intro ?toFun ?invFun
+  case toFun =>
+    unfold node
+    simp only [List.cons.injEq, Hedge.Node.mk.injEq]
+    intro ⟨ label', children', ⟨ ⟨ hlabel', hchildren' ⟩, hxs ⟩ , hif ⟩
+    subst_vars
+    simp only [and_true]
+    exact hif
+  case invFun =>
+    intro ⟨ hif , hxs  ⟩
+    unfold node
+    exists label
+    exists children
+    rw [hxs]
+    simp only [true_and]
+    exact hif
+
+theorem derive_node {α: Type} {p: α → Bool} {childlang: Lang (Hedge.Node α)} {label: α} {children: Hedge α}:
+  (Lang.derive (node p childlang) (Hedge.Node.mk label children)) =
+  (Lang.onlyif (p label /\ childlang children) Lang.emptystr) := by
+  funext
+  rw [derive_iff_node]
