Capture/Regex.lean
@@ -1,0 +1,3 @@
+import Capture.Regex.Lang
+import Capture.Regex.Map
+import Capture.Regex.Regex
