Capture/Std.lean
@@ -1,1 +1,5 @@
+import Capture.Std.Decidable
 import Capture.Std.Hedge
+import Capture.Std.List
+import Capture.Std.Vector
+import Capture.Std.Hashable
