Capture/Std/Hashable.lean
@@ -1,0 +1,7 @@
+-- A Hashable library that suppliments Lean's standard Hashable instances.
+
+instance {α: Type} {β: α -> Type} [Hashable α] [∀ a, Hashable (β a)] : Hashable (Σ (a: α), β a) where
+  hash | ⟨a, b⟩ => mixHash (hash a) (hash b)
+
+instance [Hashable α] : Hashable (Vector α n) where
+  hash | ⟨a, _⟩ => (hash a)
