Capture/Std/List.lean
@@ -1,0 +1,247 @@
+-- A List library that suppliments Lean's standard List type with extra definitions and proofs.
+
+namespace List
+
+theorem elem_lt [SizeOf α] {xs: List α} (h: x ∈ xs): sizeOf x ≤ sizeOf xs := by
+  rw [show (x ∈ xs) = List.Mem x xs from rfl] at h
+  induction h with
+  | head xs' =>
+    simp +arith only [cons.sizeOf_spec]
+  | tail _ _ ih =>
+    apply Nat.le_trans ih
+    simp +arith only [cons.sizeOf_spec, Nat.le_add_left]
+
+theorem sizeOf_cons [SizeOf α] (xs ys: List α):
+  sizeOf xs < sizeOf (y::ys ++ xs) := by
+  induction ys with
+  | nil =>
+    simp +arith only [List.cons_append, List.cons.sizeOf_spec]
+    simp only [List.nil_append, Nat.le_add_left]
+  | cons y ys ih =>
+    simp only [List.cons_append] at *
+    simp only [List.cons.sizeOf_spec] at *
+    omega
+
+theorem sizeOf_cons_lt_cons [SizeOf α] (x: α) {ys xs: List α} (h_lt: sizeOf ys < sizeOf xs):
+  sizeOf (x :: ys) < sizeOf (x :: xs) := by
+  simp only [cons.sizeOf_spec, Nat.add_lt_add_iff_left]
+  exact h_lt
+
+theorem sizeOf_lt_cons_eq [SizeOf α] (x: α) {ys xs: List α} (h_eq: ys = xs):
+  sizeOf ys < sizeOf (x :: xs) := by
+  rw [h_eq]
+  simp only [cons.sizeOf_spec, Nat.lt_add_left_iff_pos]
+  exact Nat.pos_of_neZero (1 + sizeOf x)
+
+theorem sizeOf_lt_cons_lt [SizeOf α] (x: α) {ys xs: List α} (h_lt: sizeOf ys < sizeOf xs):
+  sizeOf ys < sizeOf (x :: xs) := by
+  simp only [cons.sizeOf_spec]
+  exact Nat.lt_add_left (1 + sizeOf x) h_lt
+
+theorem length_drop_lt_cons {n: Nat} {xs: List α}:
+  (List.drop n xs).length < (x :: xs).length := by
+  simp only [length_drop, length_cons]
+  omega
+
+theorem drop_exists (n: Nat) (xs: List α): ∃ ys, xs = ys ++ (List.drop n xs) := by
+  cases n with
+  | zero =>
+    rw [drop_zero]
+    exists []
+  | succ n' =>
+    cases xs with
+    | nil =>
+      rewrite [drop_nil]
+      exists []
+    | cons x xs =>
+      simp only [List.drop_succ_cons]
+      exists (x::List.take n' xs)
+      simp only [cons_append]
+      congr
+      simp only [take_append_drop]
+
+
+-- interleaves
+
+def interleaves (xs: List α) (acc: List (List α × List α) := [([], [])])
+  : List (List α × List α) := match xs with
+  | [] => acc
+  | (x::xs) => (interleaves xs acc).map (fun res => (x::res.1, res.2))
+            ++ (interleaves xs acc).map (fun res => (res.1, x::res.2))
+
+#guard (interleaves [1,2,3,4]).contains ([1,3],[2,4])
+#guard (interleaves [1,2,3,4]).contains ([3],[1,2,4])
+#guard (interleaves [1,2,3,4]).contains ([3],[1,2,4])
+
+def interleavesAcc_length (xs: List α) (acc: List (List α × List α)): Nat :=
+  acc.length * (2 ^ xs.length)
+
+theorem interleavesAcc_length_is_correct (xs: List α) (acc: List (List α × List α)):
+  (interleaves xs acc).length = interleavesAcc_length xs acc := by
+  unfold interleavesAcc_length
+  induction xs with
+  | nil =>
+    simp only [interleaves, length_nil, Nat.pow_zero, Nat.mul_one]
+  | cons x xs ih =>
+    simp only [interleaves, length_append, length_map, length_cons]
+    rw [ih]
+    simp +arith only
+    rw [Nat.mul_left_comm]
+    rw [Nat.pow_add']
+
+def interleaves_length (xs: List α): Nat := 2 ^ xs.length
+
+theorem interleaves_length_is_correct (xs: List α):
+  (interleaves xs).length = interleaves_length xs := by
+  unfold interleaves_length
+  rw [interleavesAcc_length_is_correct]
+  unfold interleavesAcc_length
+  simp only [length_cons, length_nil, Nat.zero_add, Nat.one_mul]
+
+theorem interleaves_mem_swap (xs: List α) :
+  p ∈ interleaves xs → (p.2, p.1) ∈ interleaves xs := by
+  induction xs generalizing p with
+  | nil =>
+    intro hp
+    simp only [interleaves, mem_cons, not_mem_nil, or_false, Prod.mk.injEq] at *
+    subst hp
+    simp only [and_self]
+  | cons x xs ih =>
+    intro hp
+    simp only [interleaves, mem_append, mem_map, Prod.exists] at hp
+    rcases hp with hp | hp
+    · rcases hp with ⟨a, b, hab, heq⟩
+      simp [interleaves, interleaves, List.mem_append]
+      right
+      exists b
+      exists a
+      apply And.intro
+      · exact ih hab
+      · apply And.intro
+        · rw [←heq]
+        · rw [←heq]
+    · rcases hp with ⟨a, b, hab, heq⟩
+      simp only [interleaves, mem_append, mem_map, Prod.mk.injEq, Prod.exists,
+        exists_eq_right_right]
+      left
+      exists b
+      apply And.intro
+      · rw [←heq]
+        exact ih hab
+      · rw [←heq]
+
+theorem interleaves1_length_is_le (xs: List α):
+  ∀ ys ∈ (List.map (·.1) (interleaves xs)),
+    ys.length <= length xs
+  := by
+  intro ys hys
+  induction xs generalizing ys with
+    | nil =>
+      simp only [interleaves, map_cons, map_nil, mem_cons, not_mem_nil, or_false] at hys
+      rw [hys]
+      simp only [length_nil, Nat.le_refl]
+    | cons x xs ih =>
+      simp only [interleaves, map_append, map_map, mem_append, mem_map, Function.comp_apply,
+        Prod.exists, exists_and_right, exists_eq_right] at hys
+      simp only [mem_map, Prod.exists, exists_and_right, exists_eq_right, forall_exists_index] at ih
+      rcases hys with hys | hys
+      · rcases hys with ⟨fst, ⟨snd, hpair⟩, hys⟩
+        have hlen := ih fst snd hpair
+        rw [←hys]
+        simp only [length_cons, Nat.add_le_add_iff_right]
+        assumption
+      · rcases hys with ⟨snd, hpair⟩
+        have hlen := ih ys snd hpair
+        rw [length_cons]
+        exact Nat.le_succ_of_le hlen
+
+theorem interleaves_contains_itself_fst (xs: List α):
+  ∃ p ∈ interleaves xs, p.1 = xs := by
+  induction xs with
+  | nil =>
+    simp only [interleaves, interleaves, mem_cons, not_mem_nil, or_false, exists_eq_left]
+  | cons x xs ih =>
+    rcases ih with ⟨p, hp_mem, p_fst_eq_xs⟩
+    exists (x :: p.1, p.2)
+    constructor
+    · simp only [interleaves, mem_append, mem_map, Prod.mk.injEq, cons.injEq, true_and,
+      Prod.exists, exists_eq_right_right, exists_eq_right]
+      apply Or.inl
+      apply hp_mem
+    · simp only [cons.injEq, true_and]
+      assumption
+
+theorem interleaves_contains_itself_fst_idx (xs: List α):
+  ∃ i, ((List.interleaves xs).get i).1 = xs := by
+  have hmem := interleaves_contains_itself_fst xs
+  rcases hmem with ⟨p, hp_mem, hp_eq⟩
+  rcases (mem_iff_get).1 hp_mem with ⟨i, hi⟩
+  exists i
+  rw [hi]
+  exact hp_eq
+
+theorem interleaves_sizeOf1 (xs: List α) [SizeOf α]:
+  ∀ p ∈ interleaves xs, p.1 = xs \/ sizeOf p.1 < sizeOf xs := by
+  induction xs with
+  | nil =>
+    intro p hp
+    simp only [interleaves, mem_cons, not_mem_nil, or_false] at hp
+    left
+    rw [hp]
+  | cons x xs ih =>
+    intro p hp
+    simp only [interleaves, mem_append, mem_map, Prod.exists] at hp
+    rcases hp with hp | hp
+    · rcases hp with ⟨fst, snd, hp_mem, hp_eq⟩
+      obtain h_eq | h_lt := ih (fst, snd) hp_mem
+      · left
+        rw [←hp_eq]
+        exact congrArg (List.cons x) h_eq
+      · right
+        rw [←hp_eq]
+        exact sizeOf_cons_lt_cons x h_lt
+    · rcases hp with ⟨fst, snd, hp_mem, hp_eq⟩
+      obtain h_eq | h_lt := ih (fst, snd) hp_mem
+      · right
+        rw [←hp_eq]
+        exact sizeOf_lt_cons_eq x h_eq
+      · right
+        rw [←hp_eq]
+        exact sizeOf_lt_cons_lt x h_lt
+
+theorem interleaves_sizeOf1_idx (xs: List α) [SizeOf α] (i: Fin (List.interleaves xs).length):
+  ((List.interleaves xs).get i).1 = xs \/ sizeOf ((List.interleaves xs).get i).1 < sizeOf xs := by
+  exact interleaves_sizeOf1 xs ((interleaves xs).get i) (get_mem _ _)
+
+theorem interleaves_sizeOf2 [SizeOf α] (xs: List α):
+  ∀ p ∈ interleaves xs, p.2 = xs \/ sizeOf p.2 < sizeOf xs := by
+  induction xs with
+  | nil =>
+    intro p hp
+    simp only [interleaves, mem_cons, not_mem_nil, or_false] at hp
+    left
+    rw [hp]
+  | cons x xs ih =>
+    intro p hp
+    simp only [interleaves, mem_append, mem_map, Prod.exists] at hp
+    rcases hp with hp | hp
+    · rcases hp with ⟨fst, snd, hp_mem, hp_eq⟩
+      obtain h_eq | h_lt := ih (fst, snd) hp_mem
+      · right
+        rw [←hp_eq]
+        exact sizeOf_lt_cons_eq x h_eq
+      · right
+        rw [←hp_eq]
+        exact sizeOf_lt_cons_lt x h_lt
+    · rcases hp with ⟨fst, snd, hp_mem, hp_eq⟩
+      obtain h_eq | h_lt := ih (fst, snd) hp_mem
+      · left
+        rw [←hp_eq]
+        exact congrArg (List.cons x) h_eq
+      · right
+        rw [←hp_eq]
+        exact sizeOf_cons_lt_cons x h_lt
+
+theorem interleaves_sizeOf2_idx [SizeOf α] (xs: List α) (i: Fin (List.interleaves xs).length):
+  ((List.interleaves xs).get i).2 = xs \/ sizeOf ((List.interleaves xs).get i).2 < sizeOf xs := by
+  exact interleaves_sizeOf2 xs ((interleaves xs).get i) (get_mem _ _)
